Compiler/CompilerProof.v
@@ -1,6 +1,6 @@
 Require Import LibTactics assertion_lemmas GPUCSL TypedTerm Monad
         Host DepList CUDALib CSLLemma CSLTactics CodeGen Compiler mkMap mkReduce
-        Correctness CodeGenM SeqCompilerProof.
+        Correctness CodeGenM SeqCompilerProof Program.
 
 Definition main_spec GA :=
   let ps := gen_params GA in
@@ -9,6 +9,61 @@ Definition main_spec GA :=
      fs_tri := (All (apEnv : APtrEnv GA) (aeEnv : AEvalEnv GA),
                 FDbl (kernelInv (remove_typeinfo ps) apEnv aeEnv Emp True nil 1)
                      ((fun _ _ => True) ** (kernelInv (remove_typeinfo ps) apEnv aeEnv Emp True nil 1))) |}.
+
+Lemma genenv_ok GA : aenv_ok (remove_typeinfo (gen_params GA)).
+Proof.
+  unfold aenv_ok, gen_params.
+  generalize 0; induction GA; intros s.
+  - split; introv; inverts m.
+  - split; introv; dependent destruction m; simpl; eauto;
+    forwards* [IH1 IH2]: (IHGA (S s)).
+    clear.
+    unfold arr_name.
+    generalize 0.
+    induction a; simpl.
+    + intros ? [?|[]]; substs; simpl; eauto.
+    + intros ? [?|[]]; substs; simpl; eauto.
+    + intros ?; rewrite in_app_iff; intros [? | ?]; eauto.
+Qed.
+
+Lemma eval_compile_AE_len GA typ (arr : Skel.AE GA typ) (avenv : AVarEnv GA) (apenv : APtrEnv GA) (aeenv : AEvalEnv GA) vs :
+  Skel.aeDenote _ _ arr aeenv = Some vs
+  -> evalExp (arrInvVar avenv apenv aeenv) (compile_AE_len arr avenv) (Zn (length vs)).
+Proof.
+  unfold Skel.aeDenote.
+  dependent destruction arr; simpl.
+  intros Heq; inverts Heq.
+  - induction GA; dependent destruction m; dependent destruction avenv; dependent destruction apenv; 
+    dependent destruction aeenv; simpl; unfold arrInvVar; simpl; destruct p.
+    + evalExp.
+    + apply evalExp_app_ig, IHGA.
+  - destruct Z_le_dec; try congruence.
+    intros H; forwards*Hlen: SkelLib.mapM_length.
+    rewrite SkelLib.seq_length in Hlen.
+    rewrite Hlen.
+    rewrites* Z2Nat.id.
+    clear.
+    dependent induction l; simpl; constructor; eauto.
+    eapply alen_in.
+    instantiate (1 := snd (hget avenv m)); destruct (hget avenv m); eauto.
+Qed.
+
+Lemma hasDefval_vals typ : hasDefval (vals typ).
+Proof.
+  unfold vals; induction typ; constructor; simpl.
+  apply 0%Z.
+  apply 0%Z.
+  apply (default, default).
+Qed.
+
+Lemma flatten_aenv_avars_length GA (avenv : AVarEnv GA) :
+  length (flatten_aenv avenv) = length (flatten_avars (gen_params GA)).
+Proof.
+  unfold gen_params.
+  generalize 0.
+  induction GA; dependent destruction avenv; simpl; eauto.
+  intros n; destruct p; simpl; rewrite !app_length, !flatTup_length, (IHGA _ (S n)); eauto.
+Qed.
 
 Lemma compile_map_ok GA dom cod ntrd nblk
       (avenv : AVarEnv GA) (apenv : APtrEnv GA) (aeenv : AEvalEnv GA)
@@ -25,57 +80,57 @@ Lemma compile_map_ok GA dom cod ntrd nblk
                                                     (fst res |-> len :: snd res |=> ps) 1%Qc) Gp nil).
 Proof.
   intros Heval.
+
+  unfold Skel.skelDenote in Heval.
+  unfold bind in Heval; simpl in Heval.
+  destruct (Skel.aeDenote _ _ _ _) as [inp|] eqn:Heq1; [|inverts Heval].
+  simpl in Heval.
+  destruct (SkelLib.mapM _ inp) as [out|] eqn:Heq2; inverts Heval.
+
   unfold compile_map; simpl.
   eapply rule_backward.
   evar (ftri : FTri).
   eapply rule_bind.
   { applys (>>rule_gen_kernel).
-    skip. skip.
-    intros.
-    Definition interp_program_n_simp p fs n :=
-      interp_ftri (fs_tri fs) (fun P Q => forall ntrd nblk, CSLg_n ntrd nblk P p Q n).
-    Definition interp_program M G p fs :=
-      with_ctx M G (fun n => interp_program_n_simp p fs n).
+    3: intros; applys (>>mkMap_ok (remove_typeinfo (gen_params GA))).
+    simpl; eauto.
+    simpl; eauto.
+    apply genenv_ok. }
+  intros gen_map.
+  eapply rule_bind'.
+  { instantiate (3 := nil); simpl; eauto. }
+  apply rule_fLet.
+  { simpl; applys* eval_compile_AE_len. }
+  intros outLen.
+  eapply rule_bind'.
+  { instantiate (3 := nil); simpl; eauto. }
+  apply rule_fAllocs.
+  { evalExp. }
+  intros outs.
+  eapply rule_code_ex.
+  apply hasDefval_vals.
+  intros ps.
+  apply rule_code_ex.
+  apply listA_hasDefval.
+  intros vs.
+  apply rule_ret_back.
+  eapply rule_bind'.
+  { instantiate (1 := K (K nil)).
+    instantiate (1 := K nil).
+    instantiate (1 := nil); simpl; eauto. }
+  { eapply rule_invokeKernel.
+    - rewrite !in_app_iff; simpl; eauto.
+    - simpl; eauto.
+    - simpl; rewrite !map_app, !app_length, !map_length, !flatTup_length; eauto.
+      do 2 f_equal.
+      rewrite flatten_aenv_avars_length; eauto.
+    - repeat econstructor.
+    - do 3 (constructor; [evalExp|]).
+      rewrite map_app.
 
-    Lemma interp_fd_kfun M G k fs :
-      interp_program M G (body_of k) fs -> interp_kfun M G k fs.
-    Proof.
-      unfold interp_program, interp_kfun, with_ctx; intros Hsat n Hctx.
-      forwards* Hsat': Hsat.
-      unfold interp_program_n_simp, interp_kfun_n_simp, CSLkfun_n_simp, CSLg_n in *.
-      destruct fs as [? ? ftri]; simpl in *.
-      destruct k; simpl in *.
-      induction ftri; simpl in *; eauto.
-    Qed.
-    Lemma mkMap_ok M G GA dom cod arr_c f_c pars tag :
-      interp_kfun M G (mkMap GA dom cod arr_c f_c)
-                     (FS pars tag
-                         (All ntrd nblk avar_env aptr_env aeval_env arr f result eval_map_ok outp outs,
-                          FDbl (kernelInv avar_env aptr_env aeval_env (arrays (val2gl outp) outs 1)
-                                          True
-                                          ("nblk" |-> Zn nblk :: "ntrd" |-> Zn ntrd :: inp_len_name |-> G.Zn
-                                                  (Datatypes.length (mkMap.arr_res GA aeval_env dom cod arr f result eval_map_ok)) :: mkMap.outArr cod |=> outp) 1)
-                               (kernelInv' aptr_env aeval_env (arrays (val2gl outp) (arr2CUDA result) 1) True 1))).
-        apply interp_fd_kfun.
-        unfold interp_program, interp_program_n_simp; simpl.
-        intros n Hctx ntrd nblk avar_env aptr_env aeval_env arr f result eval_map_ok outp outs.
-        introv. 
-
-        Lemma CSLg_CSLg_n ntrd nblk P p Q : CSLg ntrd nblk P p Q -> forall n, CSLg_n ntrd nblk P p Q n.
-        Proof. unfold CSLg, CSLg_n; eauto. Qed.
-        apply CSLg_CSLg_n.
-
-
-
-
-
-          
-
-        apply mkMap_prog_ok.
-
-    apply interp_fd_kfun.
-    unfold mkMap; simpl.
-
+      apply Forall2_app.
+      
+      Lemma 
 
 
 Theorem compile_AS_ok GA ty ntrd nblk (p : Skel.AS GA ty) :
